TransVal/tvalTactics.v
@@ -4,7 +4,8 @@ Tactic Notation "setSubst" hyp(A) :=hnf in A; simpl in A; cset_tac; eapply A.
 Tactic Notation "setSubst2" hyp(A) := hnf; intros; hnf in A;  eapply A; simpl; cset_tac; eauto.
 Tactic Notation "destructBin" hyp(A) := destruct A; try destruct A;
                                         try destruct A; try destruct A; try destruct A.
-
+Tactic Notation "setSubstUnion" hyp(A) :=    intros; eapply A; unfold list_union; simpl;
+                                            eapply list_union_start_swap; cset_tac; eauto.
 (*
 *** Local Variables: ***
 *** coq-load-path: (("../" "Lvc")) ***
